src/shim.mli
@@ -49,12 +49,8 @@ module type InterpreterType = sig
   val empty_store_record : store_record
 
   (** Run one step of the interpreter. *)
-  val run_step_compat :
+  val run_one_step :
     Obj.t -> config_tuple -> res_tuple
-
-  (* Reform the one step result back to a cfg tuple, if possible *)
-  val run_step_cfg_ctx_reform:
-    config_tuple -> config_tuple option
 
   val run_v_init : 
     store_record -> administrative_instruction list -> config_tuple option
